Stlc/TypeSafety.v
@@ -79,9 +79,5 @@ Qed.
 Lemma termination_value {t τ} (wt: ⟪ empty ⊢ t : τ ⟫) :
   t⇓ → ∃ t', t -->* t' ∧ Value t'.
 Proof.
-  induction 1.
-  destruct (progress wt) as [|(t' & ?)].
-  - eauto with eval.
-  - destruct (H0 t' H1) as (t'' & vt'' & ?);
-      eauto using preservation with eval.
+  destruct 1; crush.
 Qed.
